@prefix : <http://modelmeth.nist.gov/operations#> .
@prefix owl: <http://www.w3.org/2002/07/owl#> .
@prefix rdf: <http://www.w3.org/1999/02/22-rdf-syntax-ns#> .
@prefix xml: <http://www.w3.org/XML/1998/namespace> .
@prefix xsd: <http://www.w3.org/2001/XMLSchema#> .
@prefix rdfs: <http://www.w3.org/2000/01/rdf-schema#> .

<http://modelmeth.nist.gov/operations> a owl:Ontology ;
	owl:imports <http://modelmeth.nist.gov/modeling> .
# 
# 
# #################################################################
# #
# #    Classes
# #
# #################################################################
# 
# 
# http://modelmeth.nist.gov/modeling#PredictiveModel

<http://modelmeth.nist.gov/modeling#PredictiveModel> owl:disjointWith <http://modelmeth.nist.gov/modeling#SubscriptiveModel> .
# 
# http://modelmeth.nist.gov/modeling#SubscriptiveModel
# 
# http://modelmeth.nist.gov/operations#DiscreteEventSimulation

:DiscreteEventSimulation a owl:Class ;
	rdfs:subClassOf :ModelTechnology ;
	rdfs:comment "a Monte Carlo simulation where stochastic variables are time-based." ;
	rdfs:label "Discrete Event Simulation" .
# 
# http://modelmeth.nist.gov/operations#FiniteElementMethod

:FiniteElementMethod a owl:Class ;
	rdfs:subClassOf :ModelTechnology ;
	rdfs:comment "the method of finite element analyses, a numerical technique for finding approximate solutions to boundary value problems for partial differential equations. (Wikipedia)" ;
	rdfs:label "Finite Element Method" .
# 
# http://modelmeth.nist.gov/operations#Machine

:Machine a owl:Class ;
	rdfs:subClassOf <http://modelmeth.nist.gov/modeling#Equipment> ;
	rdfs:comment "Equipment containing one or more parts that uses energy to perform an intended action. (Wikipedia)" .
# 
# http://modelmeth.nist.gov/operations#ModelTechnology

:ModelTechnology a owl:Class ;
	rdfs:subClassOf <http://modelmeth.nist.gov/modeling#ModelAbstraction> ;
	rdfs:comment "the technology used to represent the model and make inferences from it" .
# 
# http://modelmeth.nist.gov/operations#OWLClass_00002

:OWLClass_00002 a owl:Class ;
	rdfs:subClassOf <http://modelmeth.nist.gov/modeling#ModelProperty> ;
	rdfs:label "ProductionSystemProperty"@en .
# 
# http://modelmeth.nist.gov/operations#OWLClass_00003

:OWLClass_00003 a owl:Class ;
	rdfs:subClassOf <http://modelmeth.nist.gov/modeling#PerformanceVariable> , :OWLClass_00002 ;
	rdfs:comment "the number of finished products produced by the production system per unit time." ;
	rdfs:label "Throughput"@en .
# 
# http://modelmeth.nist.gov/operations#SingleJobProductionAnalyticalModel

:SingleJobProductionAnalyticalModel a owl:Class ;
	rdfs:subClassOf <http://modelmeth.nist.gov/modeling#AnalyticalModel> ;
	rdfs:comment "an AnalyticalModel of a production system describing its performance characteristics. The production system consists of a series of machines through which a single Part (job type) flow." .
# 
# 
# 
# #################################################################
# #
# #    Individuals
# #
# #################################################################
# 
# 
# http://modelmeth.nist.gov/operations#ExampleSJPmodel

:ExampleSJPmodel a owl:NamedIndividual , :SingleJobProductionAnalyticalModel .
# 
# http://modelmeth.nist.gov/operations#OWLNamedIndividual_00001

:OWLNamedIndividual_00001 a owl:NamedIndividual , :OWLClass_00003 ;
	rdfs:label "sjpModel1Throughput"@en .
# 
# http://modelmeth.nist.gov/operations#OWLNamedIndividual_00004

:OWLNamedIndividual_00004 a owl:NamedIndividual , :SingleJobProductionAnalyticalModel ;
	rdfs:label "model1"@en .
# 
# Generated by the OWL API (version 4.2.6.20160910-2108) https://github.com/owlcs/owlapi
